\documentclass[12pt,letterpaper]{article}
\usepackage{fullpage}
\usepackage[top=2cm, bottom=4.5cm, left=2.5cm, right=2.5cm]{geometry}
\usepackage{amsmath,amsthm,amsfonts,amssymb,amscd}
\usepackage{lastpage}
\usepackage{enumerate}
\usepackage{fancyhdr}
\usepackage{mathrsfs}
\usepackage{xcolor}
\usepackage{graphicx}
\usepackage{listings}
\usepackage{hyperref}
\usepackage{mathtools}
\usepackage{xfrac}
\usepackage{algorithm}
\usepackage[noend]{algpseudocode}

\hypersetup{%
  colorlinks=true,
  linkcolor=blue,
  linkbordercolor={0 0 1}
}
\linespread{1.1}
 
\renewcommand\lstlistingname{Algorithm}
\renewcommand\lstlistlistingname{Algorithms}
\def\lstlistingautorefname{Alg.}

\lstdefinestyle{Python}{
    language        = Python,
    frame           = lines, 
    basicstyle      = \footnotesize,
    keywordstyle    = \color{blue},
    stringstyle     = \color{green},
    commentstyle    = \color{red}\ttfamily
}

\setlength{\parindent}{0.0in}
\setlength{\parskip}{0.05in}

% Edit these as appropriate
\newcommand\course{Algorithms}
\newcommand\hwnumber{3}                
\newcommand\NetIDa{SUN Yilin}          
\newcommand\NetIDb{520030910361}          

\pagestyle{fancyplain}
\headheight 35pt
\lhead{\NetIDa}
\lhead{\NetIDa\\\NetIDb}           
\chead{\textbf{\Large Homework \hwnumber}}
\rhead{\course \\ \today}
\lfoot{}
\cfoot{}
\rfoot{\small\thepage}
\headsep 1.5em

\begin{document}

\section{}
\textbf{Algorithm:}\\
We sort the customers by ascending order of their service time,
then serve the customer with smallest service time each time.\\
\textbf{Proof of Correctness:}\\
The total time can be expressed as 
$$T=\sum_{i=1}^{n}\sum_{j=1}^{i}t_j$$
which is simply
$$T=\sum_{i=1}^{n}(n-i+1)t_i$$
So if the sequence $\{t_1,t_2,t_3,\dots,t_n\}$ is in ascending order, i.e.
$t_1\leq t_2\leq t_3\leq\dots\leq t_n$,
simply by the \textbf{rearrangement inequality} we know such a $T$ is the minimum waiting time
because it is the so-called "inverse product sum".\\
\newline
Below is the proof of rearrangement inequality for completeness of this problem.\\
Denote the two sequence that have already sorted by ascending order by $\{a_i\}$ and $\{b_i\}$.
Let $p_i=\sum_{j=1}^{i}b_j$, $q_i=\sum_{j=1}^{i}b_{k_j}$. It's easy to see $p_i\leq q_i$ for $i\leq n-1$ and $p_n=q_n$.\\
Then 
\begin{align}
    \sum_{i=1}^{n}a_{n-i+1}b_{i}&=\sum_{i=1}^{n-1}a_{i}(p_{n-i+1}-p_{n-i})+a_np_1\\
    &=\sum_{i=1}^{n-1}(a_{n-i+1}-a_{n-i})p_i+a_1p_n\\
    &\leq \sum_{i=1}^{n-1}(a_{n-i+1}-a_{n-i})q_i+a_1q_n\\
    &=\sum_{i=1}^{n}a_{n-i+1}b_{k_i}
\end{align}
Another side of the inequality is not used in our problem, 
so the proof is omitted here.
\end{document}
